Introduce inductive canonicalization rules

Optimizations/Canonicalization.thy
@@ -6,6 +6,102 @@ theory Canonicalization
     Proofs.Stuttering
 begin
 
+
+inductive Canonicalize_ConditionalNode :: "IRGraph \<Rightarrow> IRNode \<Rightarrow> IRNode \<Rightarrow> bool" where
+  negate_condition: (* ConditionalNode.findSynonym (252) *)
+  "\<lbrakk>kind g cond = LogicNegationNode flip\<rbrakk>
+  \<Longrightarrow> Canonicalize_ConditionalNode g (ConditionalNode cond tb fb) (ConditionalNode flip fb tb)" |
+  
+  const_true: (* ConditionalNode.findSynonym (258) *)
+  "\<lbrakk>kind g cond = ConstantNode val;
+    val_to_bool val\<rbrakk>
+  \<Longrightarrow> Canonicalize_ConditionalNode g (ConditionalNode cond tb fb) (RefNode tb)" |
+
+  const_false: (* ConditionalNode.findSynonym (256) *)
+  "\<lbrakk>kind g cond = ConstantNode val;
+    \<not>(val_to_bool val)\<rbrakk>
+  \<Longrightarrow> Canonicalize_ConditionalNode g (ConditionalNode cond tb fb) (RefNode fb)" |
+
+  eq_branches: (* ConditionalNode.canonicalizeConditional (151) *)
+  "\<lbrakk>tb = fb\<rbrakk>
+  \<Longrightarrow> Canonicalize_ConditionalNode g (ConditionalNode cond tb fb) (RefNode tb)" |
+
+  cond_eq: (* ConditionalNode.canonicalizeConditional (155) *)
+  "\<lbrakk>kind g cond = IntegerEqualsNode tb fb\<rbrakk>
+  \<Longrightarrow> Canonicalize_ConditionalNode g (ConditionalNode cond tb fb) (RefNode fb)" |
+
+  condition_bounds_x: (* ConditionalNode.canonicalizeConditional (169) *)
+  "\<lbrakk>kind g cond = IntegerLessThanNode tb fb;
+    stpi_upper (stamp g tb) \<le> stpi_lower (stamp g fb)\<rbrakk>
+  \<Longrightarrow> Canonicalize_ConditionalNode g (ConditionalNode cond tb fb) (RefNode tb)" |
+
+  condition_bounds_y: (* ConditionalNode.canonicalizeConditional (174) *)
+  "\<lbrakk>kind g cond = IntegerLessThanNode fb tb;
+    stpi_upper (stamp g fb) \<le> stpi_lower (stamp g tb)\<rbrakk>
+  \<Longrightarrow> Canonicalize_ConditionalNode g (ConditionalNode cond tb fb) (RefNode tb)"
+
+  (* ... and more *)
+
+lemma Canonicalize_ConditionalNode_Proof:
+  assumes "Canonicalize_ConditionalNode g before after"
+  assumes "g m \<turnstile> before \<mapsto> res"
+  shows "g m \<turnstile> after \<mapsto> res"
+  using assms(1) assms 
+proof (induct rule: Canonicalize_ConditionalNode.induct)
+  case (negate_condition g cond flip tb fb)
+  
+  obtain condv where condv: "g m \<turnstile> kind g cond \<mapsto> IntVal 1 condv"
+    using negate_condition.prems(2) by blast
+  then obtain flipv where flipv: "g m \<turnstile> kind g flip \<mapsto> IntVal 1 flipv"
+    by (metis LogicNegationNodeE negate_condition.hyps)
+  have invert: "condv = 0 \<longleftrightarrow> (NOT flipv) = 0"
+    using eval.LogicNegationNode condv flipv
+    by (metis Value.inject(1) evalDet negate_condition.hyps)
+  obtain tbval where tbval: "g m \<turnstile> kind g tb \<mapsto> tbval"
+    using negate_condition.prems(2) by blast
+  obtain fbval where fbval: "g m \<turnstile> kind g fb \<mapsto> fbval"
+    using negate_condition.prems(2) by blast
+  show ?case proof (cases "condv = 0")
+    case True
+    have "flipv \<noteq> 0"
+      using eval.LogicNegationNode condv flipv
+      using True evalDet negate_condition.hyps by fastforce
+    then have "fbval = res"
+      using eval.ConditionalNode tbval fbval flipv negate_condition
+      by (smt (verit, del_insts) ConditionalNodeE True Value.inject(1) condv evalDet)
+    then show ?thesis
+      by (smt (z3) ConditionalNode ConditionalNodeE \<open>flipv \<noteq> 0\<close> fbval flipv negate_condition.prems(2))
+  next
+    case False
+    have "flipv = 0"
+      using invert False sorry
+    then have "tbval = res"
+      using eval.ConditionalNode tbval fbval flipv negate_condition
+      by (smt (verit, del_insts) ConditionalNodeE False Value.inject(1) condv evalDet)
+    then show ?thesis
+      by (smt (verit, best) ConditionalNode ConditionalNodeE \<open>flipv = 0\<close> flipv negate_condition.prems(2) tbval)
+  qed
+next
+  case (const_true g cond val tb fb)
+  then show ?case sorry
+next
+  case (const_false g cond val tb fb)
+  then show ?case sorry
+next
+  case (eq_branches tb fb g cond)
+  then show ?case sorry
+next
+  case (cond_eq g cond tb fb)
+  then show ?case sorry
+next
+  case (condition_bounds_x g cond tb fb)
+  then show ?case sorry
+next
+  case (condition_bounds_y g cond fb tb)
+then show ?case sorry
+qed
+
+
 lemma add_const_nodes:
   assumes xn: "kind g x = (ConstantNode (IntVal b xv))"
   assumes yn: "kind g y = (ConstantNode (IntVal b yv))"
@@ -50,9 +146,10 @@ lemma
   assumes "x < (2 ^ LENGTH('a::len))"
   shows "sint (word_of_int x::'a word) = x"
   sorry
+*)
 
 lemma add_zero:
-  assumes "x < (2 ^ LENGTH('a)) - 1"
+  assumes "x < (2 ^ (LENGTH('a) - 1))"
   shows "(sint ((word_of_int 0::('a::len word)) + word_of_int x::('a::len word))) = x"
 proof -
   have "sint (word_of_int x::('a word)) = x"
@@ -63,8 +160,85 @@ qed
 value "word_of_int (-2)::(32word)"
 value "sint (word_of_int (-2)::32word)"
 value "sint (word_of_int 0 + word_of_int (-2)::32word)"
-*)
 
+
+(* these are incorrect with the introduction of accurate addition semantics *)
+(* most obviously due to the resultant b being either 32 or 64 *)
+lemma add_val_xzero:
+  shows "intval_add (IntVal b 0) (IntVal b yv) = (IntVal b yv)"
+  unfolding intval_add.simps sorry
+
+lemma add_val_yzero:
+  shows "intval_add (IntVal b xv) (IntVal b 0) = (IntVal b xv)"
+  unfolding intval_add.simps sorry
+
+inductive CanonicalizeAdd :: "IRGraph \<Rightarrow> IRNode \<Rightarrow> IRNode \<Rightarrow> bool" 
+  for g where
+  add_both_const:
+  "\<lbrakk>kind g x = ConstantNode c_1;
+    kind g y = ConstantNode c_2;
+    val = intval_add c_1 c_2\<rbrakk>
+    \<Longrightarrow> CanonicalizeAdd g (AddNode x y) (ConstantNode val)" |
+
+  add_xzero:
+  "\<lbrakk>kind g x = ConstantNode c_1;
+    \<not>(is_ConstantNode (kind g y));
+    c_1 = (IntVal b 0)\<rbrakk>
+    \<Longrightarrow> CanonicalizeAdd g (AddNode x y) (RefNode y)" |
+
+  add_yzero:
+  "\<lbrakk>\<not>(is_ConstantNode (kind g x));
+    kind g y = ConstantNode c_2;
+    c_2 = (IntVal b 0)\<rbrakk>
+    \<Longrightarrow> CanonicalizeAdd g (AddNode x y) (RefNode x)"
+
+lemma canonicalize_add:
+  assumes "CanonicalizeAdd g before after"
+  assumes "g m \<turnstile> before \<mapsto> res"
+  shows "g m \<turnstile> after \<mapsto> res"
+proof -
+  obtain x y where addkind: "before = AddNode x y"
+    using CanonicalizeAdd.simps assms by auto
+  from addkind
+  obtain xval where xval: "g m \<turnstile> kind g x \<mapsto> xval"
+    using assms(2) by blast
+  from addkind
+  obtain yval where yval: "g m \<turnstile> kind g y \<mapsto> yval"
+    using assms(2) by blast
+  have res: "res = intval_add xval yval"
+    using assms(2) eval.AddNode
+    using addkind evalDet xval yval by presburger
+  show ?thesis
+    using assms addkind xval yval res
+  proof (induct rule: "CanonicalizeAdd.induct")
+case (add_both_const x c_1 y c_2 val)
+  then show ?case using eval.ConstantNode by auto
+next
+  case (add_xzero x c_1 y b)
+  have xeval: "g m \<turnstile> kind g x \<mapsto> (IntVal b 0)"
+    by (simp add: ConstantNode add_xzero.hyps(1) add_xzero.hyps(3))
+  have yeval: "g m \<turnstile> kind g y \<mapsto> yval"
+    using add_xzero.prems(2) yval by fastforce
+  then have "res = intval_add (IntVal b 0) yval"
+    using eval.AddNode eval.ConstantNode add_xzero(1,3,4)
+    using evalDet by presburger
+  then show ?case using eval.RefNode yval add_val_xzero 
+    apply (cases yval; auto)
+    by (metis Value.inject(1) zero_neq_numeral)+
+next
+  case (add_yzero x y c_2 b)
+  have yeval: "g m \<turnstile> kind g y \<mapsto> (IntVal b 0)"
+    by (simp add: ConstantNode add_yzero.hyps(2) add_yzero.hyps(3))
+  have yeval: "g m \<turnstile> kind g x \<mapsto> xval"
+    using add_yzero.prems(2) xval by fastforce
+  then have "res = intval_add xval (IntVal b 0)"
+    using eval.AddNode eval.ConstantNode add_yzero(2,3,4)
+    using evalDet by presburger
+  then show ?case using eval.RefNode xval add_val_yzero 
+    apply (cases xval; auto)
+    by (metis Value.inject(1) zero_neq_numeral)+
+qed
+qed
 
 text_raw \<open>\Snip{CreateAddNode}%\<close>
 fun create_add :: "IRGraph \<Rightarrow> ID \<Rightarrow> ID \<Rightarrow> IRNode" where 
@@ -83,17 +257,6 @@ fun create_add :: "IRGraph \<Rightarrow> ID \<Rightarrow> ID \<Rightarrow> IRNod
            )
     )"
 text_raw \<open>\EndSnip\<close>
-
-
-(* these are incorrect with the introduction of accurate addition semantics *)
-(* most obviously due to the resultant b being either 32 or 64 *)
-lemma add_val_xzero:
-  shows "intval_add (IntVal b 0) (IntVal b yv) = (IntVal b yv)"
-  unfolding intval_add.simps sorry
-
-lemma add_val_yzero:
-  shows "intval_add (IntVal b xv) (IntVal b 0) = (IntVal b xv)"
-  unfolding intval_add.simps sorry
 
 
 text_raw \<open>\Snip{AddNodeCreate}%\<close>
@@ -445,28 +608,101 @@ lemma if_node_create_bisimulation:
 *)
 
 (* WIP strong bisimilar
-fun bisimilar :: "
-(IRGraph \<times> ID \<times> MapState \<times> DynamicHeap) rel
-\<Rightarrow> (IRGraph \<times> ID \<times> MapState \<times> DynamicHeap)
-\<Rightarrow> (IRGraph \<times> ID \<times> MapState \<times> DynamicHeap)
+fun strongly_bisimilar :: "
+(IRGraph \<times> ID \<times> MapState \<times> FieldRefHeap) rel
+\<Rightarrow> (IRGraph \<times> ID \<times> MapState \<times> FieldRefHeap)
+\<Rightarrow> (IRGraph \<times> ID \<times> MapState \<times> FieldRefHeap)
 \<Rightarrow> bool"
   where
-  "bisimilar \<R> (g1, nid1, m1, h1) (g2, nid2, m2, h2) =
+  "strongly_bisimilar \<R> (g1, nid1, m1, h1) (g2, nid2, m2, h2) =
     ((((g1, nid1, m1, h1), (g2, nid2, m2, h2)) \<in> \<R>) \<longrightarrow>
     ((\<forall>P'. (g1 \<turnstile> (nid1, m1, h1) \<rightarrow> P') \<longrightarrow> (\<exists>Q' . (g2 \<turnstile> (nid2, m2, h2) \<rightarrow> Q') \<and> ((g1,P'), (g2,Q')) \<in> \<R>)) \<and>
     (\<forall>Q'. (g2 \<turnstile> (nid2, m2, h2) \<rightarrow> Q') \<longrightarrow> (\<exists>P' . (g1 \<turnstile> (nid1, m1, h1) \<rightarrow> P') \<and> ((g1,P'), (g2,Q')) \<in> \<R>))))"
 *)
 
-inductive bisimilar :: "ID \<Rightarrow> IRGraph \<Rightarrow> IRGraph \<Rightarrow> bool"
+inductive weak_bisimilar :: "ID \<Rightarrow> IRGraph \<Rightarrow> IRGraph \<Rightarrow> bool"
   ("_ . _ \<sim> _") for nid where
   "\<lbrakk>\<forall>P'. (g m h \<turnstile> nid \<leadsto> P') \<longrightarrow> (\<exists>Q' . (g' m h \<turnstile> nid \<leadsto> Q') \<and> P' = Q');
     \<forall>Q'. (g' m h \<turnstile> nid \<leadsto> Q') \<longrightarrow> (\<exists>P' . (g m h \<turnstile> nid \<leadsto> P') \<and> P' = Q')\<rbrakk>
   \<Longrightarrow> nid . g \<sim> g'"
 
+text \<open>A strong bisimilution between no-op transitions\<close>
+inductive strong_noop_bisimilar :: "ID \<Rightarrow> IRGraph \<Rightarrow> IRGraph \<Rightarrow> bool"
+  ("_ | _ \<sim> _") for nid where
+  "\<lbrakk>\<forall>P'. (g \<turnstile> (nid, m, h) \<rightarrow> P') \<longrightarrow> (\<exists>Q' . (g' \<turnstile> (nid, m, h) \<rightarrow> Q') \<and> P' = Q');
+    \<forall>Q'. (g' \<turnstile> (nid, m, h) \<rightarrow> Q') \<longrightarrow> (\<exists>P' . (g \<turnstile> (nid, m, h) \<rightarrow> P') \<and> P' = Q')\<rbrakk>
+  \<Longrightarrow> nid | g \<sim> g'"
+
+lemma lockstep_strong_bisimilulation:
+  assumes "g' = replace_node nid node g"
+  assumes "g \<turnstile> (nid, m, h) \<rightarrow> (nid', m, h)"
+  assumes "g' \<turnstile> (nid, m, h) \<rightarrow> (nid', m, h)"
+  shows "nid | g \<sim> g'"
+using assms(2) assms(3) stepDet strong_noop_bisimilar.simps by blast
+
+inductive CanonicalizeIf :: "IRGraph \<Rightarrow> IRNode \<Rightarrow> IRNode \<Rightarrow> bool"
+  for g where
+  trueConst:
+  "\<lbrakk>kind g cond = ConstantNode condv;
+    val_to_bool condv\<rbrakk>
+   \<Longrightarrow> CanonicalizeIf g (IfNode cond tb fb) (RefNode tb)" |
+
+  falseConst:
+  "\<lbrakk>kind g cond = ConstantNode condv;
+    \<not>(val_to_bool condv)\<rbrakk>
+   \<Longrightarrow> CanonicalizeIf g (IfNode cond tb fb) (RefNode fb)" |
+  
+  eqBranch:
+  "\<lbrakk>\<not>(is_ConstantNode (kind g cond));
+    tb = fb\<rbrakk>
+   \<Longrightarrow> CanonicalizeIf g (IfNode cond tb fb) (RefNode tb)"
+
+lemma canonicalize_if:
+  fixes m::MapState and h::FieldRefHeap
+  assumes "kind g nid = before"
+  assumes "CanonicalizeIf g before after"
+  assumes "g' = replace_node nid (after, s) g"
+  shows "nid | g \<sim> g'"
+  using assms(2) assms 
+proof (induct rule: CanonicalizeIf.induct)
+  case (trueConst cond condv tb fb)
+  have gstep: "g \<turnstile> (nid, m, h) \<rightarrow> (tb, m, h)"
+    using ConstantNode IfNode trueConst.hyps(1) trueConst.hyps(2) trueConst.prems(1) by presburger
+  have g'step: "g' \<turnstile> (nid, m, h) \<rightarrow> (tb, m, h)"
+    using replace_node_lookup
+    by (simp add: step.RefNode trueConst.prems(3))
+  from gstep g'step show ?case
+    using lockstep_strong_bisimilulation assms(3) by simp
+next
+  case (falseConst cond condv tb fb)
+  have gstep: "g \<turnstile> (nid, m, h) \<rightarrow> (fb, m, h)"
+    using ConstantNode IfNode falseConst.hyps(1) falseConst.hyps(2) falseConst.prems(1) by presburger
+  have g'step: "g' \<turnstile> (nid, m, h) \<rightarrow> (fb, m, h)"
+    using replace_node_lookup
+    by (simp add: falseConst.prems(3) step.RefNode)
+  from gstep g'step show ?case
+    using lockstep_strong_bisimilulation assms(3) by simp
+next
+  case (eqBranch cond tb fb)
+  fix val
+  show ?case proof (cases "g m \<turnstile> kind g cond \<mapsto> val")
+    case True
+    have gstep: "g \<turnstile> (nid, m, h) \<rightarrow> (tb, m, h)"
+      using eqBranch(2,3) step.IfNode True by metis
+    have g'step: "g' \<turnstile> (nid, m, h) \<rightarrow> (tb, m, h)"
+      by (simp add: eqBranch.prems(3) step.RefNode)
+    from gstep g'step show ?thesis
+      using lockstep_strong_bisimilulation assms(3) by simp
+  next
+    case False
+    then show ?thesis sorry
+  qed
+qed
+
 lemma equal_closure_bisimilar:
   assumes "{P'. (g m h \<turnstile> nid \<leadsto> P')} = {P'. (g' m h \<turnstile> nid \<leadsto> P')}"
   shows "nid . g \<sim> g'"
-  by (metis assms bisimilar.simps mem_Collect_eq)
+  by (metis assms weak_bisimilar.simps mem_Collect_eq)
 
 
 lemma step_in_ids:
