ATVA2021/ATVA2021.thy
@@ -173,6 +173,18 @@ text_raw \<open>\Snip{AddNodeCreateDisplay}%
 @{thm[mode=Rule] add_node_create}
 \EndSnip\<close>
 
+text_raw \<open>\Snip{AddNodeRules}%
+\begin{center}
+@{thm[mode=Rule] CanonicalizeAdd.add_both_const [no_vars]}\\[8px]
+@{thm[mode=Rule] CanonicalizeAdd.add_xzero [no_vars]}\\[8px]
+@{thm[mode=Rule] CanonicalizeAdd.add_yzero [no_vars]}
+\end{center}
+\EndSnip\<close>
+
+text_raw \<open>\Snip{AddNodeProof}%
+@{thm canonicalize_add}
+\EndSnip\<close>
+
 text_raw \<open>\Snip{CreateIfNodeDisplay}%
 @{thm[display] create_if.simps}
 \EndSnip\<close>
@@ -188,6 +200,20 @@ text_raw \<open>\EndSnip\<close>
 
 text_raw \<open>\Snip{IfNodeCreateDisplay}%
 @{thm[mode=Rule] if_node_create}
+\EndSnip\<close>
+
+text_raw \<open>\Snip{CanonicalizeIfNodeRules}%
+\begin{center}
+@{thm[mode=Rule] CanonicalizeIf.trueConst}\\[8px]
+@{thm[mode=Rule] CanonicalizeIf.falseConst}\\[8px]
+@{thm[mode=Rule] CanonicalizeIf.eqBranch}
+\end{center}
+\EndSnip\<close>
+
+text_raw \<open>\Snip{CanonicalizeIfNodeProof}%
+\begin{center}
+@{thm[display] canonicalize_if}
+\end{center}
 \EndSnip\<close>
 
 (* EXPERIMENTAL *)
